SATsolver/DPLL.lean
@@ -36,6 +36,62 @@ def Formula.state.isUndecided (fs : Formula.state) : Prop :=
   | undecided _ => True
   | _ => False
 
+theorem state_undecided_undecided {f : Formula}{t : Trail} :
+  (f.getState t).isUndecided → f.undecidedBy t := by
+  simp[Formula.state.isUndecided]
+  intro h
+  split at h
+  case h_2 => contradiction
+  case h_1 fs units hund =>
+    simp[Formula.getState] at hund
+    split at hund
+    case isTrue  => contradiction
+    split at hund
+    case isTrue hsat => contradiction
+    case isFalse hcon hsat =>
+      simp at *
+      simp[Formula.undecidedBy]
+      constructor
+      case left =>
+        obtain ⟨ c, cmem, hsat ⟩ := hsat
+        have not_sat : ¬c.satisfiedBy t := by
+          split at hsat
+          contradiction
+          case h_2 s hsat' =>
+            intro contra
+            simp[Clause.getState, contra] at hsat'
+            have := Clause.sat_neq_fals contra
+            contradiction
+        have not_fals : ¬c.falsifiedBy t := by
+          have := hcon c cmem
+          split at this
+          contradiction
+          case h_2 s hcon =>
+            intro contra
+            simp[Clause.getState, contra] at hcon
+        exists c
+        constructor
+        case left => exact cmem
+        case right =>
+          apply Clause.undecided_if_not_decided
+          simp[Clause.decidedBy]
+          constructor
+          exact not_fals
+          exact not_sat
+      case right =>
+        intro c cmem
+        have not_fals : ¬c.falsifiedBy t := by
+          have := hcon c cmem
+          split at this
+          contradiction
+          case h_2 s hcon =>
+            intro contra
+            simp[Clause.getState, contra] at hcon
+        simp[Clause.fals_iff_not_sat_or_u] at not_fals
+        by_cases cu : c.undecidedBy t
+        case pos => left; exact cu
+        case neg => right; exact not_fals cu
+
 def Formula.state.units (fs : Formula.state)(wf : fs.isUndecided) : List Clause :=
   match fs with
   | undecided cs => cs
@@ -80,21 +136,21 @@ theorem Formula.getState.units_is_units {f: Formula}{t : Trail} :
 
 
 
-def SolverState.invariant (ns : List Nat)(t : Trail)(N : Nat) : Prop :=
-  ns.Nodup ∧ (∀ n ∈ ns, n ∉ t.names) ∧ (∀ n ∈ List.range N, n ∈ t.names ∨ n ∈ ns)
+def SolverState.invariant (ns : List Nat)(t : Trail)(f : Formula) : Prop :=
+  ns.Nodup ∧ (∀ n ∈ ns, n ∉ t.names) ∧ f ≠ [] ∧ f.wf ∧ (∀ n ∈ f.names, n ∈ t.names ∨ n ∈ ns)
 
 structure SolverState where
   ns : List Nat
   t : Trail
-  N : Nat
-  inv : SolverState.invariant ns t N
+  f : Formula
+  inv : SolverState.invariant ns t f
 
 
 theorem SolverState.learn_lit {s : SolverState}{a : AnnotatedLit}{wf : s.ns ≠ []} :
-  a.getName = s.ns.head wf → (unseen : a.getName ∉ s.t.names) → SolverState.invariant s.ns.tail (s.t.push a unseen) s.N := by
+  a.getName = s.ns.head wf → (unseen : a.getName ∉ s.t.names) → SolverState.invariant s.ns.tail (s.t.push a unseen) s.f := by
   intro head unseen
   simp[SolverState.invariant]
-  rcases s with ⟨ ns , t , N, inv ⟩
+  rcases s with ⟨ ns , t , f, inv ⟩
   constructor
   case left =>
     cases ns
@@ -119,44 +175,70 @@ theorem SolverState.learn_lit {s : SolverState}{a : AnnotatedLit}{wf : s.ns ≠ 
         have hmem := List.mem_of_mem_tail hmem
         exact inv.right.left m hmem
     case right =>
-      intro m hless
-      have := inv.2.2
-      simp at *
-      have := this m hless
-      cases this
-      simp[Trail.mem_names_push]
-      case inl h =>
-        simp h
-      case inr h =>
-
+      constructor
+      case left =>
+        simp
+        exact inv.2.2.1
+      constructor
+      case left =>
+        simp
+        exact  inv.2.2.2.1
+      case right =>
+        intro m hle
+        have := inv.2.2.2.2
+        simp at *
+        have := this m hle
+        simp[Trail.mem_names_push]
+        cases this
+        case inl h =>
+          left; right; exact h
+        case inr h =>
+          simp[head]
+          cases ns
+          case nil => contradiction
+          case cons x xs =>
+            simp at h ⊢
+            rcases h with h | h
+            left; left; exact h
+            right; exact h
 
 
 
 namespace DPLL
 
-def decide (s : SolverState)(l : Lit)(k : Nat)
-  (wf : s.ns ≠ [])(head : l.getName = s.ns.head wf): SolverState × Nat :=
+def decide (s : SolverState)(k : Nat)(wf : s.ns ≠ []) : SolverState :=
+  let l := Lit.pos (s.ns.head wf)
   let a := AnnotatedLit.decided l (k + 1)
   have unseen : a.getName ∉ s.t.names := by
-    have ln_mem : l.getName ∈ s.ns := by simp[head]
-    have unseen : l.getName ∉ s.t.names := s.inv.2 l.getName ln_mem
+    have ln_mem : l.getName ∈ s.ns := by simp[l, Lit.getName]
+    have unseen : l.getName ∉ s.t.names := s.inv.2.1 l.getName ln_mem
     have : a.getName = l.getName := by simp[a, AnnotatedLit.getName]
     simp[this, unseen]
   let t' := s.t.push a unseen
   let ns' := s.ns.tail
-  have inv' : SolverState.invariant ns' t' := by
+  have inv' : SolverState.invariant ns' t' s.f := by
     simp[ns', t']
     have : l.getName = a.getName := by simp[a, AnnotatedLit.getName]
-    rw[this] at head
-    exact SolverState.learn_lit head unseen
-  ( ⟨ ns', t', s.nLits, inv' ⟩, k+1 )
+    simp[l, Lit.getName] at this
+    symm at this
+    exact SolverState.learn_lit this unseen
+  ⟨ ns', t', s.f, inv' ⟩
+
+theorem decide_add_pos_decision {s : SolverState}{k : Nat}
+  {wf : s.ns ≠ []}(unseen : s.ns.head wf ∉ s.t.names):
+  (decide s k wf).t = s.t.push (AnnotatedLit.decided (Lit.pos (s.ns.head wf)) (k+1)) unseen := by
+  simp[decide]
+
+theorem decide_f_unchanged {s : SolverState}{k : Nat}{wf : s.ns ≠ []}:
+  (decide s k wf).f = s.f := by
+  simp[decide]
 
 def forget(s : SolverState)(wf : s.t.trail ≠ []): SolverState :=
   let a := s.t.trail.head wf
   let n := a.getName
   let ns' := n :: s.ns
   let t' := s.t.pop
-  have inv' : SolverState.invariant ns' t' := by
+  have inv' : SolverState.invariant ns' t' s.f := by
     simp[SolverState.invariant, ns']
     constructor
     constructor
@@ -167,23 +249,45 @@ def forget(s : SolverState)(wf : s.t.trail ≠ []): SolverState :=
         simp[AnnotatedLit.getName, Lit.getName] at this
         exact this
       intro contra
-      apply s.inv.2 n contra
+      apply s.inv.2.1 n contra
       exact this
     case left.right =>
       exact s.inv.1
-    constructor
-    case right.left =>
-      have : a = s.t.trail.head wf := by rfl
-      have : a.getName ∉ t'.names := Trail.pop_remove_head_name this
-      have hname : n = a.getName := by simp[n, AnnotatedLit.getName, Lit.getName]
-      simp[hname, this]
-    case right.right =>
-      intro m hmem contra
-      have hinv : ¬m ∈ s.t.names := s.inv.2 m hmem
-      have : t' ⊆ s.t := Trail.pop_subset
-      have : m ∈ s.t.names := Trail.names_names_subset this contra
-      contradiction
-  ⟨ ns', t', s.nLits, inv' ⟩
+    case right =>
+      constructor
+      constructor
+      case left.left =>
+        have : a = s.t.trail.head wf := by rfl
+        have : a.getName ∉ t'.names := Trail.pop_remove_head_name this
+        have hname : n = a.getName := by simp[n, AnnotatedLit.getName, Lit.getName]
+        simp[hname, this]
+      case left.right =>
+        intro m hmem contra
+        have hinv : ¬m ∈ s.t.names := s.inv.2.1 m hmem
+        have : t' ⊆ s.t := Trail.pop_subset
+        have : m ∈ s.t.names := Trail.names_names_subset this contra
+        contradiction
+      case right =>
+        constructor
+        case left =>
+          exact s.inv.2.2.1
+        constructor
+        case left =>
+          exact s.inv.2.2.2.1
+        case right =>
+          intro m hle
+          have hinv := s.inv.2.2.2.2 m hle
+          cases hinv
+          case inl hmem =>
+            have head : a = s.t.trail.head wf := by rfl
+            have := (Trail.mem_pop_ne_head_names head).right m hmem
+            simp[n, t']
+            by_cases heq : m = a.getName
+            right; left; exact heq
+            left; exact this heq
+          case inr hmem =>
+            right; right; exact hmem
+  ⟨ ns', t', s.f, inv' ⟩
 
 theorem forget_reduces {s : SolverState}{wf : s.t.trail ≠ []} :
   (forget s wf).t.trail.length < s.t.trail.length := by
@@ -204,11 +308,11 @@ def backtrack (s : SolverState) (k : Nat) : SolverState × Nat :=
     match hcase : a with
     | AnnotatedLit.decided (Lit.pos n) m =>
       let t' := s.t.negate (AnnotatedLit.decided (Lit.pos n) m) mem
-      have inv' : SolverState.invariant s.ns t' := by
+      have inv' : SolverState.invariant s.ns t' s.f := by
         simp[SolverState.invariant]
         simp[t', s.inv.1]
         exact s.inv.2
-      (⟨ s.ns, t', s.nLits, inv' ⟩, m)
+      (⟨ s.ns, t', s.f, inv' ⟩, m)
     | AnnotatedLit.decided _ m => backtrack (forget s not_nil) m
     | _ => backtrack (forget s not_nil) k
   else ⟨ s, 0 ⟩
@@ -269,69 +373,243 @@ def propogate (s : SolverState)(c : Clause)(wf : c.unitBy s.t) : SolverState :=
       exact undecided
   let ns' := s.ns.erase l.getName
   let t' := s.t.push a unseen
-  have inv' : SolverState.invariant ns' t' := by
+  have inv' : SolverState.invariant ns' t' s.f := by
     simp[ns', t', SolverState.invariant]
-    rcases s with ⟨ ns, t, _, inv ⟩
+    rcases s with ⟨ ns, t, N, inv ⟩
     constructor
     case left => exact List.nodup_erase_nodup inv.1
     case right =>
       simp
-      intro m hmem
-      simp[Trail.mem_names_push] at ⊢
       constructor
       case left =>
-        intro contra
-        have hname : l.getName = a.getName := by simp[a, AnnotatedLit.getName]
-        rw[hname, ←contra] at hmem
-        apply List.nodup_erase_self_ne_mem m inv.1
-        exact hmem
+        intro m hmem
+        simp[Trail.mem_names_push] at ⊢
+        constructor
+        case left =>
+          intro contra
+          have hname : l.getName = a.getName := by simp[a, AnnotatedLit.getName]
+          rw[hname, ←contra] at hmem
+          apply List.nodup_erase_self_ne_mem m inv.1
+          exact hmem
+        case right =>
+          have := List.mem_of_mem_erase hmem
+          exact inv.2.1 m this
       case right =>
-        have := List.mem_of_mem_erase hmem
-        exact inv.2 m this
-  ⟨ ns', t', s.nLits, inv' ⟩
+        constructor
+        case left =>
+          exact inv.2.2.1
+        constructor
+        exact inv.2.2.2.1
+        case right =>
+          intro m hle
+          have hinv := inv.2.2.2.2 m hle
+          cases hinv
+          case inl hmem =>
+            left; simp[Trail.mem_names_push]; right; exact hmem
+          case inr hmem =>
+            have : l.getName = a.getName := by simp [a, AnnotatedLit.getName]
+            rw[this]
+            by_cases heq : m = a.getName
+            case pos =>
+              left; simp [Trail.names, Trail.push]
+              left; exact heq
+            case neg =>
+              right; simp[List.mem_erase_of_ne heq, hmem]
+  ⟨ ns', t', s.f, inv' ⟩
+
 
 abbrev Distance : Type := List Nat
 
 def distanceHelper (soFar : Distance) : Nat → List AnnotatedLit → Distance
   | 0, _  => soFar
-  | n+1, [] => distanceHelper (2::soFar) n []
+  | n+1, [] => distanceHelper (soFar++[2]) n []
   | n+1, a::as => if a.isPos
-                  then distanceHelper (1::soFar) n as
-                  else distanceHelper (0::soFar) n as
+                  then distanceHelper (soFar++[1]) n as
+                  else distanceHelper (soFar++[0]) n as
+
+theorem append_sofar_append {x n : Nat}{d : Distance}{as : List AnnotatedLit} :
+  x :: distanceHelper d n as = distanceHelper (x::d) n as := by
+  induction n generalizing d as with
+  | zero => simp[distanceHelper]
+  | succ n ih =>
+    cases as
+    case nil =>
+      simp[distanceHelper]
+      apply ih
+    case cons =>
+      simp[distanceHelper]
+      split
+      case isTrue => apply ih
+      case isFalse => apply ih
 
 def Distance.distance (s : SolverState) : Distance :=
-  (distanceHelper [] s.nLits s.t.trail).reverse
+  (distanceHelper [] s.f.names.length (s.t.trail).reverse)
 
-def weightHelper (soFar : Nat) : Distance → Nat
-  | [] => soFar
-  | a :: as => weightHelper (soFar + (a * as.length)) as
+theorem mem_distance_helper_le2 {n : Nat}{soFar : Distance}{as : List AnnotatedLit}(wf : ∀ d ∈ soFar, d ≤ 2) :
+  ∀ d ∈ distanceHelper soFar n as, d ≤ 2 := by
+  intro d dh
+  induction n generalizing soFar as with
+  | zero =>
+    simp[distanceHelper] at dh
+    exact wf d dh
+  | succ n ih =>
+    have lemma: ∀ n ≤ 2, ∀ d ∈ soFar ++ [n], d ≤ 2 := by
+      simp
+      intro n nh d dh
+      cases dh
+      case inl hmem => exact wf d hmem
+      case inr heq => simp[heq, nh]
+    cases as with
+    | nil =>
+      simp[distanceHelper] at dh
+      have : ∀ (d : Nat), d ∈ soFar ++ [2] → d ≤ 2 := lemma 2 (by simp)
+      exact ih this dh
+    | cons a as =>
+      simp[distanceHelper] at dh
+      split at dh
+      case isTrue =>
+        have : ∀ (d : Nat), d ∈ soFar ++ [1] → d ≤ 2 := lemma 1 (by simp)
+        exact ih this dh
+      case isFalse =>
+        have : ∀ (d : Nat), d ∈ soFar ++ [0] → d ≤ 2 := lemma 0 (by simp)
+        exact ih this dh
 
-def Distance.weight (d : Distance): Nat :=
-  weightHelper 0 d
+
+theorem mem_distance_le2 {s : SolverState} :
+  ∀ d ∈ Distance.distance s, d ≤ 2 := by
+  simp[Distance.distance]
+  have : ∀ (n : Nat), n ∈ [] → n ≤ 2 := by simp
+  exact mem_distance_helper_le2 this
+
+
+def weightHelper (soFar : Nat) : (d : Distance) → (∀ n ∈ d, n ≤ 2) → Nat
+  | [], _ => soFar
+  | a :: as, h =>
+    have h' : (∀ n ∈ as, n ≤ 2) := by
+      intro n nh
+      have : n ∈ a::as := List.mem_cons_of_mem a nh
+      exact h n this
+    weightHelper (soFar + (a * 3 ^ (a::as).length)) as h'
+
+def Distance.weight (d : Distance)(wf : ∀ n ∈ d, n ≤ 2): Nat :=
+  weightHelper 0 d wf
 
 def Distance.lt : Distance → Distance → Prop
-  | _::_, [] => True
+  | [], [] => False
+  | _::_, [] => False
   | a::as, b::bs => if a < b then True
                     else if a = b then Distance.lt as bs
                     else False
-  | [], _ => False
+  | [], _::_ => True
 
 instance : LT Distance where
   lt as bs := Distance.lt as bs
 
+theorem distance_lt_iff_weight_lt {as bs : Distance} (aswf : ∀ a ∈ as, a ≤ 2) (bswf : ∀ b ∈ bs, b ≤ 2):
+  as < bs ↔ as.weight aswf < bs.weight bswf := by
+  constructor
+  case mp =>
+    intro h
+    induction as generalizing bs with
+    | nil =>
+      simp[Distance.weight]
+      induction bs with
+      | nil => simp[LT.lt, Distance.lt] at h
+      | cons x xs ih =>
 
-def internal(f : Formula)(s : SolverState)(k : Nat): Formula.state :=
-  let state := f.getState s.t
+
+
+
+
+theorem distance_helper_len {x y : Nat}{d : Distance}{as : List AnnotatedLit} :
+  d.length + x = y → (distanceHelper d x as).length = y := by
+  induction x generalizing d as with
+  | zero => simp[distanceHelper]
+  | succ n ih =>
+    cases as
+    case nil =>
+      simp[distanceHelper]
+      intro h
+      have : (d ++ [2]).length + n = y := by
+        simp[List.length_append, Nat.add_assoc]
+        rw[Nat.add_comm 1 n]
+        exact h
+      exact ih this
+    case cons a as =>
+      simp[distanceHelper]
+      intro h
+      split
+      case isTrue =>
+        have : (d ++ [1]).length + n = y := by
+          simp[List.length_append, Nat.add_assoc]
+          rw[Nat.add_comm 1 n]
+          exact h
+        exact ih this
+      case isFalse =>
+        have : (d ++ [0]).length + n = y := by
+          simp[List.length_append, Nat.add_assoc]
+          rw[Nat.add_comm 1 n]
+          exact h
+        exact ih this
+
+theorem distance_len_eq_n {s : SolverState} :
+  (Distance.distance s).length = s.f.names.length := by
+  simp[Distance.distance]
+  rcases s with ⟨ ns, t, f, inv⟩
+  induction f.names.length generalizing t with
+  | zero => simp[distanceHelper]
+  | succ n ih =>
+    simp at *
+    have : ([] : List Nat).length + (n + 1) = n + 1 := by simp
+    exact distance_helper_len this
+
+theorem distance_range_trail {s : SolverState} :
+  ∀ (b₁ : i < s.t.trail.length), (b₂ : i < (Distance.distance s).length) →
+  ((s.t.trail[i]'b₁).isPos → (Distance.distance s)[i]'b₂ = 1) ∧
+  (¬(s.t.trail[i]'b₁).isPos → (Distance.distance s)[i]'b₂ = 0) := by
+  intro b₁ b₂
+  simp[distance_len_eq_n] at b₂
+  constructor
+  case left =>
+    simp[Distance.distance, ]
+
+theorem distance_decide {s : SolverState}{k : Nat}{wf : s.ns ≠ []} :
+  i = (decide s k wf).t.trail.length →
+  (Distance.distance (decide s k wf))[i]? = some 1 ∧ (Distance.distance s)[i]? = some 2 ∧
+  ∀ n ≠ i, (Distance.distance (decide s k wf))[i]? = (Distance.distance s)[i]?
+  := by
+  intro h
+
+
+
+theorem state_undecided_some_undecided{s : SolverState} :
+  (s.f.getState s.t).isUndecided → s.ns ≠ [] := by
+  intro h
+  have hu := state_undecided_undecided h
+  have unseen := Formula.undecided_trail_incomplete hu s.inv.2.2.1
+  have := s.inv.2.2
+  obtain ⟨ n, nMemF, nNMemT ⟩ := unseen
+  have : n ∈ s.t.names ∨ n ∈ s.ns := s.inv.2.2.2.2 n nMemF
+  simp[nNMemT] at this
+  intro contra
+  rw[contra] at this
+  contradiction
+
+def internal(s : SolverState)(k : Nat): Formula.state :=
+  let state := s.f.getState s.t
   match hs: state with
   | .conflict =>
     let ⟨ s', k'⟩ := backtrack s k
-    if k' = 0 then state
-    else internal f s' k'
+    if backtrack s k then state
+    else internal (backtrack s k)
   | .sat => state
   | .undecided unit_cs =>
     have not_nil : s.ns ≠ [] := by
-      sorry
-    if hempty : unit_cs.isEmpty then internal f (decide s k not_nil) (k+1)
+      simp [state] at hs
+      have : (s.f.getState s.t).isUndecided := by
+        simp[Formula.state.isUndecided, hs]
+      exact state_undecided_some_undecided this
+    if hempty : unit_cs.isEmpty then internal (decide s k not_nil) (k+1)
     else
       have not_nil : unit_cs ≠ [] := by
         simp at hempty
@@ -340,7 +618,7 @@ def internal(f : Formula)(s : SolverState)(k : Nat): Formula.state :=
       have unit_head_unit : c.unitBy s.t := by
         have state_und : state.isUndecided := by
           simp[Formula.state.isUndecided, hs]
-        have : (f.getState s.t).units state_und = unit_cs := by
+        have : (s.f.getState s.t).units state_und = unit_cs := by
           simp[Formula.state.units]
           split
           case h_1 fs wf cs wf heq₁ heq=>
@@ -350,9 +628,6 @@ def internal(f : Formula)(s : SolverState)(k : Nat): Formula.state :=
         have c_mem : c ∈ unit_cs := List.head_mem not_nil
         simp[this, c_mem] at all_units
         exact all_units
-      internal f (propogate s c unit_head_unit) k
+      internal (propogate s c unit_head_unit) k
 termination_by (Distance.distance s).weight
   decreasing_by
-
-
-def dpll (f : Formula)
