SATsolver/Data/Formula.lean
@@ -5,6 +5,9 @@ abbrev Formula : Type := List Clause
 
 namespace Formula
 
+def wf (f : Formula) : Prop :=
+  f.Nodup ∧ ∀ c ∈ f, c.lits ≠ []
+
 def toStringHelper (str : String): List Clause → String
   | [] => str
   | c :: [] => str ++ s!"{c}"
@@ -12,6 +15,31 @@ def toStringHelper (str : String): List Clause → String
 
 def toString (formula : Formula) : String :=
   toStringHelper "" formula
+
+def names (f : Formula) : List Nat :=
+  (f.flatMap Clause.names)
+
+def names_no_dup (f : Formula) : List Nat := sorry
+
+theorem names_ne_nil_f_ne_nil {f : Formula}(wf : f.wf) :
+  f.names ≠ [] ↔ f ≠ [] := by
+  simp [names]
+  constructor
+  case mp =>
+    intro h contra
+    obtain ⟨ c, cmem, cunseen ⟩ := h
+    rw[contra] at cmem
+    contradiction
+  case mpr =>
+    intro h
+    cases f
+    case nil => contradiction
+    case cons c cs =>
+      exists c
+      simp[Clause.names]
+      exact wf.2 c List.mem_cons_self
+
+
 
 end Formula
 
