SATsolver/Experiment/DPLL/backtrack.lean
@@ -1,0 +1,46 @@
+import SATsolver.Experiment.Relations.Theories
+
+def backtrack (t : Trail)(wf : ∃ a ∈ t, a.decidedP) : Trail :=
+  have : t ≠ [] := by
+    intro contra
+    simp[contra] at wf
+  match t with
+  | a::as =>
+    match a with
+    | .decided l => (ALit.deduced l.negate)::as
+    | .deduced _ =>
+      have : (∃ a ∈ as, a.decidedP) := by
+        obtain ⟨ a, amem, adec ⟩ := wf
+        rw[ALit.dec_is_dec] at adec
+        obtain ⟨ l, ha ⟩ := adec
+        simp [ha] at amem
+        exists a
+        simp[ha, amem, ALit.decidedP]
+      backtrack as this
+
+theorem backtrack_lemma {hd tl : Trail}{a : ALit}{wf: ∃ e ∈ (hd++a::tl), e.decidedP} :
+  (∀ e ∈ hd, ¬ e.decidedP) → a.decidedP → backtrack (hd++a::tl) wf = (ALit.deduced a.lit.negate)::tl := by
+  intro hhd ha
+  cases a
+  case deduced => simp[ALit.decidedP] at ha
+  case decided l =>
+    induction hd
+    case nil =>
+      simp[backtrack, ALit.lit]
+    case cons x xs ih =>
+      have hhd2 : (∀ (e : ALit), e ∈ xs → ¬e.decidedP) := by
+        intro a amem
+        have : a ∈ x::xs := by simp[List.mem_cons, amem]
+        exact hhd a this
+      have wf2 : ∃ e, e ∈ xs ++ (ALit.decided l)::tl ∧ e.decidedP := by
+        obtain ⟨ e, emem, he ⟩ := wf
+        cases emem
+        case head => have := hhd x; simp at this; contradiction
+        case tail hmem => exists e
+      cases x
+      case decided l =>
+        have := hhd (ALit.decided l)
+        simp[ALit.decidedP] at this
+      case deduced =>
+        simp[backtrack]
+        exact ih hhd2
