SATsolver/Experiment/DPLL/decide.lean
@@ -1,0 +1,4 @@
+import SATsolver.Experiment.Relations.Theories
+
+def dec (l : Lit)(t : Trail)(_ : t ¿ l): Trail :=
+  ALit.decided l :: t
