SATsolver/Experiment/DPLL/distance.lean
@@ -1,0 +1,249 @@
+import SATsolver.Experiment.Relations.Theories
+import SATsolver.Experiment.DPLL.misc
+import SATsolver.Experiment.DPLL.decide
+import SATsolver.Experiment.DPLL.propogate
+import SATsolver.Experiment.DPLL.backtrack
+
+/- Distance is a measure used to prove termination. The idea is that the first
+differing element in a reversed trail decides the distance. For example a trail
+with a deduced last element has always a smaller distance than a trail without-/
+
+def distance_internal (soFar : Nat) : Trail → Nat → Nat
+  | _, 0 => soFar
+  | [], n+1 => distance_internal (soFar + 2*3^n) [] n
+  | (ALit.decided _)::as, n+1 => distance_internal (soFar + 1*3^n) as n
+  | (ALit.deduced _)::as, n+1 =>  distance_internal soFar as n
+
+def distance_partial (soFar stop : Nat) : Trail → Nat → Nat
+  | t, n =>
+    if n ≤ stop then soFar
+    else match t, n with
+      | _, 0 => soFar
+      | [], n+1 => distance_partial (soFar + 2 * 3 ^ n) stop [] n
+      | (ALit.decided _) :: as, n+1 => distance_partial (soFar + 1 * 3 ^ n) stop as n
+      | (ALit.deduced _) :: as, n+1 => distance_partial soFar stop as n
+
+def distance(t : Trail)(f : Formula)(_ : f ≠ []) : Nat :=
+  distance_internal 0 t.reverse f.names.eraseDups.length
+
+theorem extract_soFar {soFar n: Nat}{t : Trail}(x : Nat):
+  distance_internal (soFar + x ) t n = soFar + distance_internal x t n := by
+  induction n generalizing soFar x t with
+  | zero => simp[distance_internal]
+  | succ n ih =>
+    cases t
+    case nil => simp [distance_internal, Nat.add_assoc, ih]
+    case cons a as =>
+      cases a
+      case decided a => simp [distance_internal, Nat.add_assoc, ih]
+      case deduced a => simp [distance_internal, ih]
+
+theorem extract_x {soFar n: Nat}{t : Trail}(x : Nat):
+  distance_internal (soFar + x ) t n = x + distance_internal soFar t n := by
+  induction n generalizing soFar x t with
+  | zero => simp[distance_internal, Nat.add_comm]
+  | succ n ih =>
+    cases t
+    case nil => simp [distance_internal, Nat.add_assoc, ih]
+    case cons a as =>
+      cases a
+      case decided a => simp [distance_internal, Nat.add_assoc, ih]
+      case deduced a => simp [distance_internal, ih]
+
+theorem extract_from_partial {t} {soFar n s}(x) :
+  distance_partial (soFar + x ) s t n = soFar + distance_partial x s t n := by
+  induction n generalizing soFar t x s
+  case zero => simp[distance_partial]
+  case succ n ih =>
+    cases t
+    case nil =>
+      simp[distance_partial]
+      split
+      case isTrue => rfl
+      case isFalse => simp[Nat.add_assoc, ih]
+    case cons a as =>
+      cases a
+      case decided a =>
+        simp[distance_partial]
+        split
+        case isTrue => rfl
+        case isFalse => simp[Nat.add_assoc, ih]
+      case deduced a =>
+        simp [distance_partial]
+        split
+        case isTrue => rfl
+        case isFalse => simp[ih]
+
+theorem distance_partial_zero {soFar n}{t} :
+  distance_partial soFar 0 t n = distance_internal soFar t n := by
+  induction n generalizing soFar t
+  case zero => simp[distance_internal, distance_partial]
+  case succ k ih =>
+    cases t
+    case nil => simp[distance_internal, distance_partial, ih]
+    case cons a as =>
+      cases a
+      case decided l => simp[distance_internal, distance_partial, ih]
+      case deduced l =>  simp[distance_internal, distance_partial, ih]
+
+theorem distance_partial_n {soFar n}{t} :
+  distance_partial soFar n t n = soFar := by
+  unfold distance_partial
+  simp
+
+theorem split_internal {soFar n}{hd tl : Trail} :
+  hd.length ≤ n → distance_internal soFar (hd++tl) n = distance_partial 0 (n-hd.length) hd n + distance_partial soFar 0 tl (n-hd.length) := by
+  intro hlt
+  induction hd generalizing n
+  case nil => simp[distance_partial_n, distance_partial_zero]
+  case cons x xs ih =>
+    cases n
+    case zero => simp at hlt
+    case succ n =>
+      cases x
+      case decided =>
+        simp[distance_internal, distance_partial]
+        split
+        case isTrue htrue =>
+          have h1 : n - xs.length ≤ n := Nat.sub_le n xs.length
+          have h2 : n < n + 1 := Nat.lt_succ_self n
+          have := Nat.lt_of_le_of_lt h1 h2
+          have := Nat.lt_le_asymm this
+          contradiction
+        case isFalse hfalse =>
+          simp at hlt
+          have : distance_partial (3 ^ n) (n - xs.length) xs n = (3 ^ n) + distance_partial 0 (n - xs.length) xs n := extract_from_partial 0
+          simp[extract_x, this, ih hlt]
+          simp +arith
+      case deduced =>
+        simp[distance_internal, distance_partial]
+        split
+        case isTrue htrue =>
+          have h1 : n - xs.length ≤ n := Nat.sub_le n xs.length
+          have h2 : n < n + 1 := Nat.lt_succ_self n
+          have := Nat.lt_of_le_of_lt h1 h2
+          have := Nat.lt_le_asymm this
+          contradiction
+        case isFalse hfalse =>
+          simp at hlt
+          simp[ih hlt]
+
+theorem soFar_lt {x y n: Nat}{t : Trail}:
+  x < y → distance_internal x t n < distance_internal y t n := by
+  intro h
+  have h1 : distance_internal x t n = x + distance_internal 0 t n := extract_soFar 0
+  have h2 : distance_internal y t n = y + distance_internal 0 t n := extract_soFar 0
+  rw[h1, h2]
+  simp[h]
+
+theorem distance_append {soFar n : Nat}{as: Trail}{a : ALit}:
+  n > as.length → distance_internal soFar (as++[a]) n < distance_internal soFar as n := by
+  induction as generalizing soFar n with
+  | nil =>
+    cases n with
+    | zero => simp
+    | succ n =>
+      cases a
+      case decided =>
+        simp[distance_internal]
+        have : soFar + 3 ^ n < soFar + 2 * 3 ^ n := by simp[arith_helper]
+        simp[soFar_lt this]
+      case deduced =>
+        simp[distance_internal]
+        have : soFar < soFar + 2 * 3 ^ n := by
+            simp
+            rw[←Nat.ne_zero_iff_zero_lt]
+            simp[Nat.pow_eq_zero]
+        simp[soFar_lt this]
+  | cons b as ih =>
+    intro h
+    rw[List.length_cons] at h
+    have : n ≠ 0 := by
+      intro contra
+      rw[contra] at h
+      contradiction
+    obtain ⟨ m, hm ⟩ := Nat.exists_eq_succ_of_ne_zero this
+    have : m > as.length := by
+      simp[hm] at h ⊢
+      exact h
+    cases b
+    case decided => simp[hm, distance_internal, ih this]
+    case deduced => simp[hm, distance_internal, ih this]
+
+theorem helper {soFar n : Nat }{t : Trail} :
+  distance_internal soFar t n < soFar + 3^n := by
+  induction n generalizing t
+  case zero => simp[distance_internal]
+  case succ n ih =>
+    cases t
+    case nil =>
+      simp[distance_internal, Nat.pow_succ]
+      rw[Nat.add_comm]
+      have : distance_internal (2 * 3 ^ n + soFar ) [] n = 2 * 3 ^ n + distance_internal (soFar) [] n := extract_soFar soFar
+      rw[this]
+      simp +arith
+      exact ih
+    case cons hd tl =>
+      cases hd
+      case deduced =>
+        simp[distance_internal, Nat.pow_succ]
+        have h₁ := ih (t := tl)
+        apply Nat.lt_of_lt_of_le h₁
+        simp +arith
+      case decided =>
+        simp[distance_internal, Nat.pow_succ]
+        have : distance_internal (3 ^ n + soFar ) tl n = 3 ^ n + distance_internal (soFar) tl n := extract_soFar soFar
+        rw[Nat.add_comm, this]
+        simp +arith
+        have h₁ := ih (t := tl)
+        apply Nat.lt_of_lt_of_le h₁
+        simp +arith
+
+theorem head_subst{soFar n : Nat}{t y : Trail}{l j : Lit}:
+  n ≠ 0 → distance_internal soFar ((ALit.deduced l)::y) n < distance_internal soFar ((ALit.decided j)::t) n := by
+  intro nh
+  obtain ⟨ k, kh ⟩ := Nat.exists_eq_succ_of_ne_zero nh
+  simp[kh, distance_internal]
+  have : distance_internal (soFar + 3 ^ k) t k = (soFar + 3 ^ k) + distance_internal 0 t k := extract_soFar 0
+  rw[this]
+  apply Nat.lt_add_right
+  exact helper
+
+theorem distance_dec {l : Lit}{t : Trail}{f : Formula}{lud : t ¿ l}{wf : f ≠ []}:
+  f.names.eraseDups.length > t.length → distance (dec l t lud) f wf < distance t f wf:= by
+  intro h
+  simp only [distance, dec, List.reverse_cons]
+  apply distance_append
+  simp[h]
+
+theorem distance_prop{t : Trail}{c : Clause}{pwf : c.unit t}{f : Formula}{wf : f ≠ []}:
+  f.names.eraseDups.length > t.length → distance (propogate t c pwf) f wf < distance t f wf:= by
+  intro h
+  simp only [distance, propogate, List.reverse_cons]
+  apply distance_append
+  simp[h]
+
+theorem distance_bc{t : Trail}{bcwf : ∃ a ∈ t, a.decidedP}{f : Formula}{wf : f ≠ []}:
+  f.names.eraseDups.length > t.length → distance (backtrack t bcwf) f wf < distance t f wf := by
+  intro h
+  obtain ⟨ hd, tl, a, heq, ha, hhd ⟩ := exists_split_on_prop ALit.decidedP t bcwf
+  subst heq
+  have : backtrack (hd ++ a :: tl) bcwf = ALit.deduced (a.lit.negate)::tl := backtrack_lemma hhd ha
+  simp[this, distance]
+  have hle : tl.reverse.length < f.names.eraseDups.length := by
+    simp at h ⊢
+    have : tl.length + 1 < f.names.eraseDups.length := Nat.lt_of_add_left_lt h
+    exact Nat.lt_of_add_right_lt this
+  rw[split_internal, split_internal]
+  simp[distance_partial_zero]
+  cases a
+  case deduced => simp[ALit.decidedP] at ha
+  case decided l =>
+    have : f.names.eraseDups.length - tl.length ≠ 0 := by
+      apply Nat.ne_of_gt
+      simp at hle
+      exact Nat.sub_pos_of_lt hle
+    simp only[ALit.lit]
+    exact head_subst this
+  exact Nat.le_of_lt hle
+  exact Nat.le_of_lt hle
