SATsolver/Experiment/DPLL/impl.lean
@@ -1,0 +1,63 @@
+import SATsolver.Experiment.Relations.Theories
+import SATsolver.Experiment.DPLL.distance
+
+def internal (t : Trail)(f : Formula)(wf : f ≠ []): Bool :=
+  if sat : decide (t ⊨ f) then
+    true
+  else if con : decide (t ⊭ f) then
+    if anyDec : t.any ALit.decidedB then
+      have bcwf : ∃ a ∈ t, a.decidedP := by
+        simp[ALit.decidedP_iff_decidedB] at anyDec
+        obtain ⟨ a, amem, adec ⟩ := anyDec
+        exists a
+      internal (backtrack t bcwf) f wf
+    else false
+  else
+    let copt := f.find? (fun c => c.unit t)
+    if h : copt.isSome then
+      let c := copt.get h
+      have : c.unit t := by
+        have cunit : copt = some c := by
+          simp[c]
+        simp[copt] at cunit
+        have := List.find?_some cunit
+        simp at this
+        exact this
+      internal (propogate t c this) f wf
+    else
+      have ud : t¿f := by
+        simp at *
+        exact Formula.nSatCon_ud sat con
+      let copt := (f.find? (t¿·))
+      have : copt.isSome := by
+        have := Formula.ud_iff_exists_csUD.mp ud
+        simp[copt, this]
+      let c := copt.get this
+      have : t ¿ c := by
+        have heq : copt = some c := by
+          simp[c]
+        simp[copt] at heq
+        have := List.find?_some heq
+        simp at this
+        exact this
+      let lopt := (c.find? (t¿·))
+      have : lopt.isSome := by
+        have := Clause.ud_exists_lUd this
+        simp[lopt, this]
+      let l := lopt.get this
+      have : t ¿ l := by
+        have heq : lopt = some l := by
+          simp[l]
+        simp[lopt] at heq
+        have := List.find?_some heq
+        simp at this
+        exact this
+      internal (dec l t this) f wf
+termination_by distance t f wf
+decreasing_by
+  have : f.names.eraseDups.length > t.length := by sorry
+  exact distance_bc this
+  have : f.names.eraseDups.length > t.length := by sorry
+  exact distance_prop this
+  have : f.names.eraseDups.length > t.length := by sorry
+  exact distance_dec this
