SATsolver/Experiment/DPLL/misc.lean
@@ -1,0 +1,28 @@
+theorem exists_split_on_prop{α : Type _} (p : α → Prop)(t : List α)(h : ∃ e ∈ t, p e) :
+    ∃ hd tl a, t = hd ++ a :: tl ∧ p a ∧ ∀ x ∈ hd, ¬ p x := by
+    induction t
+    case nil => simp at h
+    case cons x xs ih =>
+      by_cases hx : p x
+      case pos =>
+        exists [], xs
+        simp[hx]
+      case neg =>
+        have : (∃ e, e ∈ xs ∧ p e) := by
+          obtain ⟨ e, hmem, he ⟩ := h
+          cases hmem
+          case head => contradiction
+          case tail hmem => exists e
+        obtain ⟨ hd, tl, a, h ⟩ := ih this
+        exists (x::hd), tl, a
+        simp[hx, h]
+        intro b bmem
+        exact h.2.2 b bmem
+
+theorem arith_helper {n : Nat} :
+  3 ^ n < 2 * 3 ^ n := by
+  induction n
+  case zero => simp
+  case succ n ih =>
+    rw[Nat.pow_succ, ←Nat.mul_assoc]
+    simp[ih]
