SATsolver/Experiment/DPLL/propogate.lean
@@ -1,0 +1,5 @@
+import SATsolver.Experiment.Relations.Theories
+
+def propogate (t : Trail)(c : Clause)(wf : c.unit t): Trail :=
+  let l := c.getunit t wf
+  ALit.deduced l :: t
