SATsolver/Experiment/Data/ALit.lean
@@ -1,0 +1,61 @@
+import SATsolver.Experiment.Data.Lit
+
+inductive ALit where
+  | decided : Lit → ALit
+  | deduced : Lit  → ALit
+
+namespace ALit
+
+def lit : ALit → Lit
+  | decided l => l
+  | deduced l  => l
+
+instance : Coe ALit Lit where
+  coe a := a.lit
+
+def negate : ALit → ALit
+  | decided l => decided l.negate
+  | deduced l  => decided l.negate
+
+def decidedP : ALit → Prop
+  | decided _ => True
+  | deduced _ => False
+
+def decidedB : ALit → Bool
+  | decided _ => true
+  | deduced _ => false
+
+def deducedP : ALit → Prop
+  | decided _ => False
+  | deduced _ => True
+
+def deduceB : ALit → Bool
+  | decided _ => false
+  | deduced _ => true
+
+theorem decidedP_iff_decidedB (a : ALit) :
+  decidedB a = true ↔ decidedP a := by
+  simp[decidedP, decidedB]
+  split
+  all_goals simp
+
+instance : DecidablePred decidedP :=
+  fun
+  | decided _ => isTrue trivial
+  | deduced _ => isFalse (by simp [decidedP])
+
+theorem dec_is_dec {a : ALit}:
+    a.decidedP ↔ ∃ l, a = decided l := by
+    simp[decidedP]
+    split
+    all_goals simp
+
+def name : ALit → Nat
+  | decided l | deduced l => l.name
+
+theorem name_name_lit {a : ALit} :
+  a.lit.name = a.name := by
+  simp only [name, lit, Lit.name]
+  rcases a with ⟨ l ⟩ | ⟨ l ⟩
+  all_goals cases l
+  all_goals simp
