SATsolver/Experiment/Data/Clause.lean
@@ -1,0 +1,29 @@
+import SATsolver.Experiment.Data.Trail
+
+abbrev Clause : Type := List Lit
+
+namespace Clause
+
+def names (c : Clause) : List Nat := c.map Lit.name
+
+theorem mem_mem_name {c : Clause}{l : Lit} :
+  l ∈ c → l.name ∈ c.names := by
+  intro mem
+  simp[names]
+  exists l
+
+theorem mem_names_exist_mem {c : Clause}{n : Nat} :
+  n ∈ c.names → ∃ l, l.name = n ∧ l ∈ c := by
+  simp[names]
+  intro l lmem lname
+  exists l
+
+def wf (c : Clause) : Prop :=
+  c ≠ [] ∧ ∀ l1 ∈ c, ∀ l2 ∈ c, l1 ≠ l2 → l1.name ≠ l2.name
+
+
+theorem wf_names {c : Clause} :
+  c.wf → c.names ≠ [] := by
+  simp[wf, names]
+  intro nNil _
+  exact nNil
