SATsolver/Experiment/Data/Formula.lean
@@ -1,0 +1,80 @@
+import SATsolver.Experiment.Data.Clause
+
+abbrev Formula : Type := List Clause
+
+namespace Formula
+
+def lits (f : Formula) : List Lit := f.flatten
+
+def wf(f : Formula) : Prop := ∀ c ∈ f, c.wf
+
+def mem_memClause_mem {f : Formula}{c : Clause} :
+  c ∈ f → ∀ l ∈ c, l ∈ f.lits := by
+  intro mem l lmem
+  induction f with
+  | nil => contradiction
+  | cons x xs ih =>
+    cases mem
+    case head =>
+      simp[lits]
+      left; exact lmem
+    case tail mem =>
+      have mem : c ∈ xs := mem
+      have := ih mem
+      simp[lits] at ⊢ this
+      right; exact this
+
+
+def names (f : Formula) : List Nat := (f.flatMap Clause.names)
+
+def names_cons {f : Formula}(wf : f.wf) :
+  f ≠ [] → f.names ≠ [] := by
+  intro h
+  rw[List.ne_nil_iff_exists_cons] at h
+  obtain ⟨ c, cs, h ⟩ := h
+  subst h
+  simp[names, Clause.names]
+  intro falsity
+  have : c ≠ [] := by
+    simp[Formula.wf, Clause.wf] at wf
+    simp[wf]
+  contradiction
+
+
+def mem_memClause_mem_names {f : Formula}{c : Clause}{n : Nat} :
+  c ∈ f → n ∈ c.names → n ∈ f.names := by
+  intro mem nmem
+  induction f with
+  | nil => contradiction
+  | cons x xs ih =>
+    cases mem
+    case head =>
+      simp[names]
+      left; exact nmem
+    case tail mem =>
+      have mem : c ∈ xs := mem
+      have := ih mem
+      simp[names] at ⊢ this
+      right; exact this
+
+instance : Membership Clause Formula where
+  mem f c := c ∈ f
+
+instance : Membership Lit Formula where
+  mem f l := ∃ c ∈ f, l ∈ c
+
+end Formula
+
+namespace variables
+
+abbrev variables : Type := Nat
+
+-- Checks that all the variables is in a formula
+-- and that the formula contains all the vars
+def wf (vs : variables)(f : Formula) : Prop :=
+  (∀ n ∈ f.names, n ≤ vs) ∧ (∀ n ≤ vs, n ∈ f.names)
+
+instance : DecidableRel wf := by
+  intro vs f
+  simp[wf]
+  exact instDecidableAnd
