SATsolver/Experiment/Data/Lit.lean
@@ -1,0 +1,57 @@
+inductive Lit where
+  | pos : Nat → Lit
+  | neg : Nat → Lit
+
+namespace Lit
+
+instance : BEq Lit where
+  beq x y := match x, y with
+    | pos x, pos y => x == y
+    | neg x, neg y => x == y
+    | _, _ => false
+
+instance : LawfulBEq Lit where
+  rfl := by
+    intro a
+    simp[BEq.beq]
+    cases a
+    all_goals simp
+  eq_of_beq := by
+    intro a b h
+    simp[BEq.beq] at h
+    cases a <;> cases b
+    case pos.pos | neg.neg =>
+      simp at h
+      simp[h]
+    case pos.neg | neg.pos =>
+      simp at h
+
+instance : DecidableEq Lit := by
+  intro a b
+  cases a <;> cases b
+  case pos.pos a b | neg.neg a b =>
+    simp
+    exact Nat.decEq a b
+  all_goals
+    exact isFalse (by intro h; cases h)
+
+
+def negate : Lit → Lit
+  | pos n => neg n
+  | neg n => pos n
+
+def name : Lit → Nat
+  | pos n | neg n => n
+
+theorem name_name_negate {l : Lit} :
+  l.negate.name = l.name := by
+  simp[negate, name]
+  cases l
+  all_goals simp
+
+theorem shared_name {a b : Lit} :
+  a.name = b.name → a = b ∨ a = b.negate := by
+  simp[name]
+  intro h
+  cases a <;> cases b
+  all_goals simp[h, negate]
