SATsolver/Experiment/Data/Trail.lean
@@ -1,0 +1,31 @@
+import SATsolver.Experiment.Data.ALit
+
+abbrev Trail : Type := List ALit
+
+namespace Trail
+
+def lits : Trail → List Lit
+  | t => t.map ALit.lit
+
+theorem mem_mem_lits{t : Trail}{a : ALit} :
+  a ∈ t → a.lit ∈ t.lits := by
+  simp[lits]
+  intro h
+  exists a
+
+def names : Trail → List Nat
+  |t => t.map ALit.name
+
+theorem mem_name_exists_mem {t : Trail}{n : Nat} :
+  n ∈ t.names → ∃ a ∈ t, a.name = n := by
+  simp[names]
+
+def unseen (t : Trail)(n : Nat) : Prop := n ∉ t.names
+
+instance : DecidableRel unseen :=
+  fun t n => inferInstanceAs (Decidable (n ∉ t.names))
+
+def wf (t : Trail) : Prop := t.names.Nodup
+
+instance : DecidablePred Trail.wf :=
+  fun t => List.nodupDecidable (t.names)
