SATsolver/Experiment/Relations/Conflicts.lean
@@ -1,0 +1,34 @@
+import SATsolver.Experiment.Data.Formula
+
+class Conflict (α β : Type) where
+  con : α → β → Prop
+
+infix:50 "⊭" => Conflict.con
+
+instance : Conflict Trail Lit where
+  con t l := l.negate ∈ t.lits
+
+instance : DecidableRel (Conflict.con (α := Trail) (β := Lit)) := by
+  intro t l
+  simp[Conflict.con]
+  apply List.instDecidableMemOfLawfulBEq
+
+instance : Conflict Trail Clause where
+  con t c := ∀ l ∈ c, t ⊭ l
+
+instance : DecidableRel (Conflict.con (α := Trail) (β := Clause)) := by
+    intro t c
+    simp[Conflict.con]
+    apply List.decidableBAll
+
+instance : Conflict Trail Formula where
+  con t f := ∃ c ∈ f, t ⊭ c
+
+instance : DecidableRel (Conflict.con (α := Trail) (β := Formula)) := by
+  intro t f
+  simp[Conflict.con]
+  apply List.decidableBEx
+
+def Formula.con_iff_exists_csCon {f : Formula}{t : Trail} :
+  t ⊭ f ↔ ∃ c ∈ f, t ⊭ c := by
+  simp[Conflict.con]
