SATsolver/Experiment/Relations/Satisfies.lean
@@ -1,0 +1,45 @@
+import SATsolver.Experiment.Data.Formula
+
+class Satisfies (α β : Type) where
+  sat : α → β → Prop
+
+infix:50 "⊨" => Satisfies.sat
+
+instance : Satisfies Lit Clause where
+  sat l c := l ∈ c
+
+instance : DecidableRel (Satisfies.sat (α := Lit) (β := Clause)) :=
+  fun l c => List.instDecidableMemOfLawfulBEq l c
+
+instance : Satisfies ALit Clause where
+  sat a c := a.lit ∈ c
+
+instance : DecidableRel (Satisfies.sat (α := ALit) (β := Clause)) :=
+  fun a c => List.instDecidableMemOfLawfulBEq a.lit c
+
+theorem Clause.mem_entails {l : Lit}{c : Clause}:
+  l ∈ c ↔ l ⊨ c := by simp[Satisfies.sat]
+
+instance : Satisfies Trail Lit where
+  sat t l := l ∈ t.lits
+
+instance : DecidableRel (Satisfies.sat (α := Trail) (β := Lit)) := by
+  intro t l
+  simp[Satisfies.sat]
+  apply List.instDecidableMemOfLawfulBEq
+
+instance : Satisfies Trail Clause where
+  sat t c := ∃ l ∈ c, t ⊨ l
+
+instance : DecidableRel (Satisfies.sat (α := Trail) (β := Clause)) :=
+  fun t c => c.decidableBEx ( t ⊨ .)
+
+instance : Satisfies Trail Formula where
+  sat t f := ∀ (c : Clause), c ∈ f → t ⊨ c
+
+instance : DecidableRel (Satisfies.sat (α := Trail) (β := Formula)) :=
+  fun t f => (f.decidableBAll (t ⊨ .))
+
+def Formula.sat_iff_all_csSat {f : Formula}{t : Trail} :
+  t ⊨ f ↔ ∀ c ∈ f, t ⊨ c := by
+  simp[Satisfies.sat]
