SATsolver/Experiment/Relations/Theories.lean
@@ -1,0 +1,67 @@
+import SATsolver.Experiment.Relations.Satisfies
+import SATsolver.Experiment.Relations.Conflicts
+import SATsolver.Experiment.Relations.Undecided
+
+theorem Clause.ud_exUnseen{c : Clause}{t : Trail}:
+  t¿c → ∃ l ∈ c, t.unseen l.name := by
+  simp[Undecided.ud]
+  intro l lmem lunseen cud
+  exists l
+
+theorem Formula.ud_exCUd{f : Formula}{t : Trail}:
+  t¿f → f ≠ [] := by
+  cases f
+  all_goals simp[Undecided.ud]
+
+theorem Formula.Clause.ud_exUnseen{f : Formula}{t : Trail}:
+  t¿f → ∃ n ∈ f.names, t.unseen n := by
+  simp [Undecided.ud, Formula.names]
+  intro c cmem l lmem lunseen ohters
+  have cn : l.name ∈ c.names := Clause.mem_mem_name lmem
+  have fn : l.name ∈ f.names := Formula.mem_memClause_mem_names cmem cn
+  exists l.name
+  constructor
+  case left => exists c
+  case right =>  simp[Trail.unseen, lunseen]
+
+theorem Clause.nSatCon_ud{c : Clause}{t : Trail}:
+   ¬ t ⊭ c → ¬t ⊨ c → t¿c := by
+  simp[Satisfies.sat, Conflict.con, Undecided.ud]
+  intro l lmem lncon nsat
+  have lnsat := nsat l lmem
+  constructor
+  case left =>
+    exists l
+    constructor
+    case left => exact lmem
+    case right =>
+      intro contra
+      obtain ⟨ a, amem, aname ⟩ := Trail.mem_name_exists_mem contra
+      rw[←ALit.name_name_lit] at aname
+      have litmem := Trail.mem_mem_lits amem
+      cases Lit.shared_name aname
+      case inl heq => rw[heq] at litmem; contradiction
+      case inr heq => rw[heq] at litmem; contradiction
+  case right =>
+    intro k kmem
+    have := nsat k kmem
+    by_cases kcon : k.negate ∈ t.lits
+    case pos => simp[kcon]
+    case neg =>
+      left
+      intro contra
+      obtain ⟨ a, amem, aname ⟩ := Trail.mem_name_exists_mem contra
+      rw[←ALit.name_name_lit] at aname
+      have litmem := Trail.mem_mem_lits amem
+      cases Lit.shared_name aname
+      case inl heq => rw[heq] at litmem; contradiction
+      case inr heq => rw[heq] at litmem; contradiction
+
+
+theorem Formula.nSatCon_ud{f : Formula}{t : Trail}:
+  ¬t ⊨ f → ¬ t ⊭ f → t¿f := by
+  simp[Formula.sat_iff_all_csSat, Formula.con_iff_exists_csCon, Formula.ud_iff_exists_csUD]
+  intro c cmem ncSat ncon
+  have ncCon := ncon c cmem
+  have := Clause.nSatCon_ud ncCon ncSat
+  exists c
