SATsolver/Experiment/Relations/Undecided.lean
@@ -1,0 +1,60 @@
+import SATsolver.Experiment.Data.Formula
+import SATsolver.Experiment.Relations.Conflicts
+
+class Undecided (α β : Type) where
+  ud : α → β → Prop
+
+infix:50 "¿" => Undecided.ud
+
+instance : Undecided Trail Lit where
+  ud t l := l.name ∉ t.names
+
+instance : DecidableRel (Undecided.ud (α := Trail) (β := Lit)) := by
+  intro t l
+  simp[Undecided.ud, Lit.name, Trail.names]
+  apply List.decidableBAll
+
+instance : Undecided Trail Clause where
+  ud t c := (∃ l' ∈ c, t¿l') ∧ (∀ l ∈ c, t¿l ∨ t⊭l)
+
+instance : DecidableRel (Undecided.ud (α := Trail) (β := Clause)) := by
+  intro a b
+  simp[Undecided.ud]
+  apply instDecidableAnd
+
+theorem Clause.ud_exists_lUd{c : Clause}{t : Trail} :
+  t ¿ c → ∃ l ∈ c, t ¿ l := by
+  simp[Undecided.ud]
+  intro l lmem lunseen _
+  exists l
+
+
+def Clause.unit (c :Clause)(t : Trail) : Prop :=
+   ∃ l' ∈ c, t¿l' ∧ ∀ l ∈ c, l ≠ l' → t ⊭ l
+
+instance : DecidableRel Clause.unit := by
+  intro c t
+  simp[Clause.unit]
+  apply List.decidableBEx
+
+def Clause.getunit (c :Clause)(t : Trail)(wf : c.unit t) : Lit :=
+  let lopt := c.find? (fun l => t ¿ l)
+  have : lopt.isSome := by
+    simp only [Clause.unit] at wf
+    obtain ⟨ l, hmem, hud, cCon ⟩ := wf
+    simp[lopt]
+    exists l
+  lopt.get this
+
+instance : Undecided Trail Formula where
+  ud t f := ∃ c ∈ f, t¿c
+
+instance : DecidableRel (Undecided.ud (α := Trail) (β := Formula)) := by
+  intro a b
+  simp[Undecided.ud]
+  apply List.decidableBEx
+
+
+def Formula.ud_iff_exists_csUD {f : Formula}{t : Trail} :
+  t ¿ f ↔ ∃ c ∈ f, t ¿ c := by
+  simp[Undecided.ud]
